Giving up on universal type approach. Trying a less informative value type, after discussion with Michael.

hol/ptypesScript.sml
@@ -1,81 +1,157 @@
-open HolKernel bossLib boolLib boolSimps Parse pairTheory optionTheory stringTheory finite_mapTheory sumTheory state_transformerTheory option_transformerTheory monadsyntax lcsymtacs
+open HolKernel bossLib boolLib boolSimps SatisfySimps Parse pairTheory optionTheory stringTheory finite_mapTheory sumTheory state_transformerTheory option_transformerTheory monadsyntax lcsymtacs
 
 val _ = new_theory "ptypes"
 
+val _ = Hol_datatype `ptr = addr of 'a itself => num`;
+val num_to_ptr_def = Define `num_to_ptr n = addr (:'a) n`;
+val ptr_to_num_def = Define `ptr_to_num (addr _ n) = n`;
+val _ = export_rewrites ["num_to_ptr_def","ptr_to_num_def"];
+val _ = overload_on("pnil",``addr ARB 0``);
+
 val _ = type_abbrev ("varname",``:string``);
 val _ = type_abbrev ("funname",``:string``);
-val _ = Hol_datatype `ptr = pnil of 'a | addr of num`;
-
 val _ = Hol_datatype `AuxList = <| head : 'a ptr ; tail : AuxList ptr |>`;
-val _ = Hol_datatype `List = <| first : 'a AuxList ptr ; last : 'a AuxList ptr |> ` ;
+val _ = Hol_datatype `List = <| first : 'a AuxList ptr ; last : 'a AuxList ptr |>` ;
 
-val _ = Hol_datatype `
+val _ = Hol_datatype`
   SetOfVariables = <| counter : num ; varnumb : num ; vars : Variable List ptr |> ;
   Multiequation = <| erased : bool ; S : SetOfVariables ptr ; M : (VarTerm + FunTerm) List ptr |> ;
   Variable = <| name : varname ; m : Multiequation ptr |> ;
   FunTerm = <| fsymb : funname ; args : (VarTerm + FunTerm) List ptr |> ;
-  VarTerm = <| v : Variable ptr |> ` ;
+  VarTerm = <| v : Variable ptr |>`;
 val _ = type_abbrev("Term", ``:(VarTerm + FunTerm)``);
 val _ = Hol_datatype `TempMultiequation = <| S : Term List ptr ; M : Term List ptr |>`;
 val _ = Hol_datatype `System = <| T : Multiequation List ptr ; U : Multiequation List ptr |>`;
 
-val _ = type_abbrev ("value",
-``:Variable
- + SetOfVariables
- + Term
- + Term AuxList
- + Term List
- + Multiequation
- + Multiequation AuxList
- + Multiequation List
- + TempMultiequation
- + TempMultiequation AuxList
- + TempMultiequation List
- + System``);
+val _ = Hol_datatype `
+value = Variable_value of varname => num
+      | SetOfVariables_value of num => num => num
+      | Term_value of num + funname # num
+      | Multiequation_value of bool => num => num
+      | TempMultiequation_value of num => num
+      | System_value of num => num
+      | AuxList_value of num => num
+      | List_value of num => num`;
+
+val _ = type_abbrev("inject", ``:'a -> value``);
+val _ = type_abbrev("project", ``:value -> 'a option``);
+val _ = type_abbrev("embed", ``:'a inject # 'a project``);
+val inject_Variable_def = Define`
+  inject_Variable a = Variable_value a.name (ptr_to_num a.m)`;
+val project_Variable_def = Define`
+  (project_Variable (Variable_value name vars) = SOME (Variable name (num_to_ptr vars))) ∧
+  (project_Variable _ = NONE)`;
+val _ = overload_on("embed_Variable",``(inject_Variable, project_Variable)``);
+val inject_SetOfVariables_def = Define`
+  inject_SetOfVariables a = SetOfVariables_value a.counter a.varnumb (ptr_to_num a.vars)`;
+val project_SetOfVariables_def = Define`
+  (project_SetOfVariables (SetOfVariables_value counter varnumb vars) = SOME (SetOfVariables counter varnumb (num_to_ptr vars))) ∧
+  (project_SetOfVariables _ = NONE)`;
+val _ = overload_on("embed_SetOfVariables",``(inject_SetOfVariables, project_SetOfVariables)``);
+val inject_Term_def = Define`
+  (inject_Term (INL al) = Term_value (INL (ptr_to_num al.v))) ∧
+  (inject_Term (INR ar) = Term_value (INR (ar.fsymb, (ptr_to_num ar.args))))`;
+val project_Term_def = Define`
+  (project_Term (Term_value (INL v)) = SOME (INL (VarTerm (num_to_ptr v)))) ∧
+  (project_Term (Term_value (INR (fsymb, args))) = SOME (INR (FunTerm fsymb (num_to_ptr args)))) ∧
+  (project_Term _ = NONE)`;
+val _ = overload_on("embed_Term",``(inject_Term, project_Term)``);
+val inject_Multiequation_def = Define`
+  inject_Multiequation a = Multiequation_value a.erased (ptr_to_num a.S) (ptr_to_num a.M)`;
+val project_Multiequation_def = Define`
+  (project_Multiequation (Multiequation_value erased S_ M) = SOME (Multiequation erased (num_to_ptr S_) (num_to_ptr M))) ∧
+  (project_Multiequation _ = NONE)`;
+val _ = overload_on("embed_Multiequation",``(inject_Multiequation, project_Multiequation)``);
+val inject_TempMultiequation_def = Define`
+  inject_TempMultiequation a = TempMultiequation_value (ptr_to_num a.S) (ptr_to_num a.M)`;
+val project_TempMultiequation_def = Define`
+  (project_TempMultiequation (TempMultiequation_value S_ M) = SOME (TempMultiequation (num_to_ptr S_) (num_to_ptr M))) ∧
+  (project_TempMultiequation _ = NONE)`;
+val _ = overload_on("embed_TempMultiequation",``(inject_TempMultiequation, project_TempMultiequation)``);
+val inject_System_def = Define`
+  inject_System a = System_value (ptr_to_num a.T) (ptr_to_num a.U)`;
+val project_System_def = Define`
+  (project_System (System_value T_ U) = SOME (System (num_to_ptr T_) (num_to_ptr U))) ∧
+  (project_System _ = NONE)`;
+val _ = overload_on("embed_System",``(inject_System, project_System)``);
+val inject_AuxList_def = Define`
+  inject_AuxList a = AuxList_value (ptr_to_num a.head) (ptr_to_num a.tail)`;
+val project_AuxList_def = Define`
+  (project_AuxList (AuxList_value head tail) = SOME (AuxList (num_to_ptr head) (num_to_ptr tail))) ∧
+  (project_AuxList _ = NONE)`;
+val _ = overload_on("embed_AuxList",``(inject_AuxList, project_AuxList)``);
+val inject_List_def = Define`
+  inject_List a = List_value (ptr_to_num a.first) (ptr_to_num a.last)`;
+val project_List_def = Define`
+  (project_List (List_value first last) = SOME (List (num_to_ptr first) (num_to_ptr last))) ∧
+  (project_List _ = NONE)`;
+val _ = overload_on("embed_List",``(inject_List, project_List)``);
+val _ = export_rewrites["inject_Variable_def","project_Variable_def","inject_SetOfVariables_def","project_SetOfVariables_def","inject_Term_def","project_Term_def","inject_Multiequation_def","project_Multiequation_def","inject_TempMultiequation_def","project_TempMultiequation_def","inject_System_def","project_System_def","inject_AuxList_def","project_AuxList_def","inject_List_def","project_List_def"];
+
+val is_embed_def = Define`
+  is_embed ((i,p):'a embed) = ∀a. p (i a) = SOME a`;
+local
+  fun Cases_on_rhs (g as (asl,tm)) = let
+    val (_,rhs) = dest_eq tm
+    val var = if is_var rhs then rhs else snd (dest_comb rhs)
+  in Cases_on [QUOTE (term_to_string var)] end g
+  val tac = srw_tac [][is_embed_def] >> rpt (Cases_on_rhs >> srw_tac [][])
+in
+  val is_embed_Variable = Q.store_thm("is_embed_Variable", `is_embed embed_Variable`, tac);
+  val is_embed_SetOfVariables = Q.store_thm("is_embed_SetOfVariables", `is_embed embed_SetOfVariables`, tac);
+  val is_embed_Term = Q.store_thm("is_embed_Term", `is_embed embed_Term`, tac);
+  val is_embed_Multiequation = Q.store_thm("is_embed_Multiequation", `is_embed embed_Multiequation`, tac);
+  val is_embed_TempMultiequation = Q.store_thm("is_embed_TempMultiequation", `is_embed embed_TempMultiequation`, tac);
+  val is_embed_System = Q.store_thm("is_embed_System", `is_embed embed_System`, tac);
+  val is_embed_AuxList = Q.store_thm("is_embed_AuxList", `is_embed embed_AuxList`, tac);
+  val is_embed_List = Q.store_thm("is_embed_List", `is_embed embed_List`, tac);
+end
 
 val _ = type_abbrev("store", ``:num |-> value``);
 
-val embed_def = Define`
-  embed = @p. ∀x. (SND p) ((FST p) x : value) = x`
-val _ = overload_on ("inject", ``FST embed``);
-val _ = overload_on ("eject", ``SND embed``);
+val raw_lookup_def = Define`
+  raw_lookup ((i,p):'a embed) (addr _ n : 'a ptr) = OPTIONT_BIND (λs. (FLOOKUP s n, s)) (λv. UNIT (p v))`;
+val _ = overload_on("lookup", ``λp:Variable ptr. raw_lookup embed_Variable p``);
+val _ = overload_on("lookup", ``λp:SetOfVariables ptr. raw_lookup embed_SetOfVariables p``);
+val _ = overload_on("lookup", ``λp:Term ptr. raw_lookup embed_Term p``);
+val _ = overload_on("lookup", ``λp:Multiequation ptr. raw_lookup embed_Multiequation p``);
+val _ = overload_on("lookup", ``λp:TempMultiequation ptr. raw_lookup embed_TempMultiequation p``);
+val _ = overload_on("lookup", ``λp:System ptr. raw_lookup embed_System p``);
+val _ = overload_on("lookup", ``λp:'a AuxList ptr. raw_lookup embed_AuxList p``);
+val _ = overload_on("lookup", ``λp:'a List ptr. raw_lookup embed_List p``);
 
-val embed_Term_thm = Q.store_thm(
-"embed_Term_thm",
-`eject (inject (v:Term)) = v`,
-srw_tac [][embed_def] >>
-SELECT_ELIM_TAC >> srw_tac [][] >>
-qexists_tac `(INR o INR o INL, OUTL o OUTR o OUTR)` >>
-srw_tac [][]);
-
-val embed_Term_List_thm = Q.store_thm(
-"embed_Term_List_thm",
-`eject (inject (v:Term List)) = v`,
-srw_tac [][embed_def] >>
-SELECT_ELIM_TAC >> srw_tac [][] >>
-qexists_tac `(INR o INR o INR o INR o INL, OUTL o OUTR o OUTR o OUTR o OUTR)` >>
-srw_tac [][]);
-
-val lookup_def = Define`
-  (lookup (addr n : 'a ptr) = OPTIONT_BIND (λs. (FLOOKUP s n, s)) (λv. OPTIONT_UNIT (eject:value->'a v))) ∧
-  (lookup pnil_ = OPTIONT_FAIL)`;
-
-val assign_def = Define`
-  (assign (addr n : 'a ptr) v = (λs:store. ((), s |+ (n, inject:'a->value v)))) ∧
-  (assign pnil_ v = return ())`;
+val raw_assign_def = Define`
+  raw_assign ((i,p):'a embed) (addr _ n : 'a ptr) v = λs:store. ((), s |+ (n, i v))`;
+val _ = overload_on("assign", ``λp:Variable ptr. raw_assign embed_Variable p``);
+val _ = overload_on("assign", ``λp:SetOfVariables ptr. raw_assign embed_SetOfVariables p``);
+val _ = overload_on("assign", ``λp:Term ptr. raw_assign embed_Term p``);
+val _ = overload_on("assign", ``λp:Multiequation ptr. raw_assign embed_Multiequation p``);
+val _ = overload_on("assign", ``λp:TempMultiequation ptr. raw_assign embed_TempMultiequation p``);
+val _ = overload_on("assign", ``λp:System ptr. raw_assign embed_System p``);
+val _ = overload_on("assign", ``λp:'a AuxList ptr. raw_assign embed_AuxList p``);
+val _ = overload_on("assign", ``λp:'a List ptr. raw_assign embed_List p``);
 
 val dispose_def = Define`
-  (dispose (addr n) = (λs:store. ((), s \\ n))) ∧
-  (dispose _ = return ())`;
+  dispose (addr _ n) = λs:store. ((), s \\ n)`;
 
 val free_addr_def = Define`
-  free_addr = λs:store. (addr (@n. n ∉ FDOM s), s)`;
+  free_addr = λs:store. (addr ARB (@n. n ≠ 0 ∧ n ∉ FDOM s), s)`;
 
-val new_def = Define`new v = do ptr <- free_addr ; assign ptr v ; return ptr od`;
+val raw_new_def = Define`raw_new emb v = do ptr <- free_addr ; raw_assign emb ptr v ; return ptr od`;
+val _ = overload_on("new", ``λv:Variable. raw_new embed_Variable v``);
+val _ = overload_on("new", ``λv:SetOfVariables. raw_new embed_SetOfVariables v``);
+val _ = overload_on("new", ``λv:Term. raw_new embed_Term v``);
+val _ = overload_on("new", ``λv:Multiequation. raw_new embed_Multiequation v``);
+val _ = overload_on("new", ``λv:TempMultiequation. raw_new embed_TempMultiequation v``);
+val _ = overload_on("new", ``λv:System. raw_new embed_System v``);
+val _ = overload_on("new", ``λv:'a AuxList. raw_new embed_AuxList v``);
+val _ = overload_on("new", ``λv:'a List. raw_new embed_List v``);
+
+val _ = export_rewrites["raw_lookup_def","raw_assign_def","dispose_def","raw_new_def"];
 
 val CreateList_def = Define`
   CreateList =
-  do l <- new (AuxList (pnil ARB) (pnil ARB)) ;
+  do l <- new (AuxList pnil pnil) ;
      s <- new (List l l) ;
      return s
   od`;
@@ -105,7 +181,7 @@ val TailOfList_def = Define`
 
 val AddToEndOfList_def = Define`
   AddToEndOfList t s =
-  do l <- new (AuxList (pnil ARB) (pnil ARB)) ;
+  do l <- new (AuxList pnil pnil) ;
      s' <- lookup s ;
      assign s'.last (AuxList t l) ;
      assign s (List s'.first l) ;
@@ -137,14 +213,14 @@ val AppendLists_def = Define`
   od`;
 
 val (corresponding_list_rules, corresponding_list_ind, corresponding_list_cases) = Hol_reln`
-  (((EmptyList ptr) s = (SOME T, s')) ⇒ corresponding_list ptr s []) ∧
+  (((EmptyList ptr) s = (SOME T, s')) ⇒ corresponding_list emb ptr s []) ∧
   (((do hd <- HeadOfList ptr ;
         tl <- TailOfList ptr ;
-        (hd':'a) <- lookup hd ;
+        (hd':'a) <- raw_lookup emb hd ;
         return (hd',tl)
      od) s = (SOME (hd',tl),s')) ∧
-   corresponding_list tl s' tl' ⇒
-   corresponding_list ptr s (hd'::tl'))`;
+   corresponding_list emb tl s' tl' ⇒
+   corresponding_list emb ptr s (hd'::tl'))`;
 
 val NOTIN_INFINITE_FDOM_exists = Q.store_thm(
 "NOTIN_INFINITE_FDOM_exists",
@@ -154,72 +230,75 @@ val _ = export_rewrites["NOTIN_INFINITE_FDOM_exists"];
 
 val free_addr_elim_thm = Q.store_thm(
 "free_addr_elim_thm",
-`∀P s. (∀n. n ∉ FDOM s ⇒ P (addr n,s)) ⇒ P (free_addr s)`,
+`∀P s. (∀n. n ≠ 0 ∧ n ∉ FDOM s ⇒ P (addr ARB n,s)) ⇒ P (free_addr s)`,
 srw_tac [][free_addr_def] >>
 SELECT_ELIM_TAC >>
-srw_tac [][]);
+`∃x. x ∉ FDOM (s|+(0,ARB))` by srw_tac [][] >>
+fsrw_tac [SATISFY_ss][]);
+
+val _ = augment_srw_ss [rewrites [BIND_DEF,IGNORE_BIND_DEF,UNIT_DEF,OPTIONT_BIND_def,OPTIONT_FAIL_def,OPTIONT_UNIT_def]]
 
 val CreateList_creates_empty = Q.store_thm(
 "CreateList_creates_empty",
-`(∀v. eject (inject (v:'a List)) = v) ⇒ (CreateList s0 = (ptr : 'a List ptr, s)) ⇒ corresponding_list ptr s []`,
-strip_tac >>
-simp_tac (srw_ss()) [CreateList_def,new_def,BIND_DEF] >>
+`(CreateList s0 = (ptr : 'a List ptr, s)) ⇒ corresponding_list emb ptr s []`,
+simp_tac (srw_ss()) [CreateList_def,raw_new_def] >>
 qho_match_abbrev_tac `(UNCURRY f (UNCURRY g (free_addr s0)) = (ptr,s)) ⇒ X` >>
 Q.ABBREV_TAC `P = (λx. (UNCURRY f (UNCURRY g x) = (ptr,s)) ⇒ X)` >>
 qsuff_tac `P (free_addr s0)` >- srw_tac [][Abbr`P`] >>
 ho_match_mp_tac free_addr_elim_thm >>
-srw_tac [][Abbr`P`,Abbr`g`,Abbr`f`,IGNORE_BIND_DEF,BIND_DEF,UNIT_DEF,assign_def,UNCURRY,Abbr`X`] >>
-Q.ABBREV_TAC `P = (λx. corresponding_list (FST x) (SND (assign (FST x) (List (addr n) (addr n)) (SND x))) [])`  >>
-qsuff_tac `P (free_addr (s0 |+ (n,inject (AuxList (pnil (ARB:'a)) (pnil ARB)))))` >- srw_tac [][Abbr`P`] >>
+srw_tac [][Abbr`P`,Abbr`g`,Abbr`f`,UNCURRY,Abbr`X`] >>
+Q.ABBREV_TAC `P = (λx. corresponding_list emb (FST x) (SND (assign (FST x) (List (addr ARB n) (addr ARB n)) (SND x))) [])`  >>
+qsuff_tac `P (free_addr (s0 |+ (n,AuxList_value 0 0)))` >- srw_tac [][Abbr`P`] >>
 ho_match_mp_tac free_addr_elim_thm >>
-srw_tac [][Abbr`P`,assign_def,Once corresponding_list_cases,EmptyList_def,OPTIONT_BIND_def,BIND_DEF,lookup_def,OPTIONT_UNIT_def,UNIT_DEF,FLOOKUP_UPDATE]);
+srw_tac [][Abbr`P`,Once corresponding_list_cases,EmptyList_def,FLOOKUP_UPDATE]);
 
+(* only true for "well-formed" stores that don't bind 0. But maybe lookup should have this property for all stores anyway?
 val lookup_pnil = Q.store_thm(
 "lookup_pnil",
-`lookup (pnil a) s = (NONE, s)`,
-srw_tac [][lookup_def,OPTIONT_FAIL_def,UNIT_DEF]);
+`lookup pnil s = (NONE, s)`,
+srw_tac [][]);
 val _ = export_rewrites ["lookup_pnil"];
+*)
 
 val lookup_preserves_store = Q.store_thm(
 "lookup_preserves_store",
-`SND (lookup ptr s) = s`,
-Cases_on `ptr` >> srw_tac [][lookup_def,OPTIONT_FAIL_def,OPTIONT_UNIT_def,UNIT_DEF,OPTIONT_BIND_def,BIND_DEF,FLOOKUP_DEF]);
+`SND (raw_lookup emb ptr s) = s`,
+Cases_on `emb` >> Cases_on `ptr` >> srw_tac [][FLOOKUP_DEF]);
 
 val HeadOfList_preserves_store = Q.store_thm(
 "HeadOfList_preserves_store",
 `SND (HeadOfList l s) = s`,
 `SND (lookup l s) = s` by MATCH_ACCEPT_TAC lookup_preserves_store >>
-srw_tac [][HeadOfList_def,OPTIONT_BIND_def,BIND_DEF,lookup_preserves_store,OPTIONT_FAIL_def,OPTIONT_UNIT_def,UNIT_DEF,UNCURRY] >>
+srw_tac [][HeadOfList_def,lookup_preserves_store,UNCURRY] >>
 Cases_on `FST (lookup l s)` >> srw_tac [][] >>
 `SND (lookup x.first s) = s` by MATCH_ACCEPT_TAC lookup_preserves_store >>
 srw_tac [][UNCURRY] >>
 Cases_on `FST (lookup x.first s)` >> srw_tac [][]);
 
+(* same as lookup_pnil
 val HeadOfList_pnil = Q.store_thm(
 "HeadOfList_pnil",
 `HeadOfList (pnil a) s = (NONE, s)`,
 srw_tac [][HeadOfList_def,OPTIONT_BIND_def,UNIT_DEF,BIND_DEF]);
 val _ = export_rewrites["HeadOfList_pnil"];
+*)
 
+(* same as lookup_pnil
 val TailOfList_pnil = Q.store_thm(
 "TailOfList_pnil",
 `TailOfList (pnil a) s = (NONE, s)`,
 srw_tac [][TailOfList_def,OPTIONT_BIND_def,BIND_DEF,UNIT_DEF]);
 val _ = export_rewrites["TailOfList_pnil"];
+*)
 
 val TailOfList_preserves_store = Q.store_thm(
 "TailOfList_preserves_store",
-`(lookup (addr n : 'a List ptr) s = (SOME l', s')) ∧ (l'.first = addr m) ⇒ (SND (TailOfList (addr n : 'a List ptr) s) \\ n \\ m = s \\ n \\ m)`,
-srw_tac [][TailOfList_def,OPTIONT_BIND_def,BIND_DEF,UNCURRY,UNIT_DEF,assign_def,dispose_def,OPTIONT_UNIT_def] >>
+`(lookup l s = (SOME l', s')) ⇒ (SND (TailOfList l s) \\ (ptr_to_num l) \\ (ptr_to_num l'.first) = s \\ (ptr_to_num l) \\ (ptr_to_num l'.first))`,
+srw_tac [][TailOfList_def,UNCURRY] >>
 `s' = s` by PROVE_TAC [lookup_preserves_store,SND] >>
-`SND (lookup (addr m : 'a AuxList ptr) s) = s` by PROVE_TAC [lookup_preserves_store,SND] >>
-Cases_on `FST (lookup (addr m : 'a AuxList ptr) s)` >> srw_tac [][IGNORE_BIND_DEF,BIND_DEF] >>
-srw_tac [][DOMSUB_IDEM,DOMSUB_COMMUTES] >>
-PROVE_TAC [DOMSUB_COMMUTES,DOMSUB_FUPDATE]);
-
-val DOMSUB_FLOOKUP_NEQ = Q.store_thm(
-"DOMSUB_FLOOKUP_NEQ",
-`k1 ≠ k2 ⇒ (FLOOKUP (fm \\ k1) k2 = FLOOKUP fm k2)`,
-srw_tac [][FLOOKUP_DEF,DOMSUB_FAPPLY_NEQ]);
+`SND (lookup l'.first s) = s` by PROVE_TAC [lookup_preserves_store,SND] >>
+Cases_on `FST (lookup l'.first s)` >> srw_tac [][] >>
+Cases_on `l` >> Cases_on `l'.first` >>
+srw_tac [][DOMSUB_COMMUTES]);
 
 val _ = export_theory ()
